utp/utp_dynlog.thy
@@ -79,7 +79,7 @@ lemma sBoxTest [dynlog_intro]: "\<Gamma> \<tturnstile> (b \<Rightarrow> \<Psi>) 
   by (rel_auto)
 
 lemma sBoxAssignFwd [dynlog_intro]: 
-  assumes "vwb_lens x" "\<And> x\<^sub>0. ((\<Gamma>\<lbrakk>\<guillemotleft>x\<^sub>0\<guillemotright>/&x\<rbrakk> \<and> &x =\<^sub>u v\<lbrakk>\<guillemotleft>x\<^sub>0\<guillemotright>/&x\<rbrakk>) \<tturnstile> \<Phi>)"
+  assumes "vwb_lens x" "\<And> x\<^sub>0. ((\<Gamma>\<lbrakk>\<guillemotleft>x\<^sub>0\<guillemotright>/&x\<rbrakk> \<and> &x = v\<lbrakk>\<guillemotleft>x\<^sub>0\<guillemotright>/&x\<rbrakk>) \<tturnstile> \<Phi>)"
   shows "(\<Gamma> \<tturnstile> \<^bold>[x := v\<^bold>]\<Phi>)"
 proof -
   have "\<lbrace>\<Gamma>\<rbrace> x := v ;; II \<lbrace>\<Phi>\<rbrace>\<^sub>u"
@@ -88,7 +88,7 @@ proof -
     by (simp add: hoare_as_dynlog)
 qed
 
-lemma sBoxAssignFwd_simp [dynlog_simp]: "\<lbrakk> vwb_lens x; x \<sharp> v; x \<sharp> \<Gamma> \<rbrakk> \<Longrightarrow> (\<Gamma> \<tturnstile> \<^bold>[x := v\<^bold>]\<Phi>) = ((&x =\<^sub>u v \<and> \<Gamma>) \<tturnstile> \<Phi>)"
+lemma sBoxAssignFwd_simp [dynlog_simp]: "\<lbrakk> vwb_lens x; x \<sharp> v; x \<sharp> \<Gamma> \<rbrakk> \<Longrightarrow> (\<Gamma> \<tturnstile> \<^bold>[x := v\<^bold>]\<Phi>) = ((&x = v \<and> \<Gamma>) \<tturnstile> \<Phi>)"
   by (rel_auto, metis vwb_lens_wb wb_lens.get_put)
 
 lemma sBoxIndStar: "\<tturnstile> [\<Phi> \<Rightarrow> \<^bold>[P\<^bold>]\<Phi>]\<^sub>u \<Longrightarrow> \<Phi> \<tturnstile> \<^bold>[P\<^sup>\<star>\<^bold>]\<Phi>"
