utp/utp_sequent.thy
@@ -7,6 +7,8 @@ begin
 definition sequent :: "'\<alpha> upred \<Rightarrow> '\<alpha> upred \<Rightarrow> bool" (infixr "\<tturnstile>" 15) where
 [upred_defs]: "sequent P Q = (Q \<sqsubseteq> P)"
 
+utp_lift_notation sequent
+
 abbreviation sequent_triv ("\<tturnstile> _" [15] 15) where "\<tturnstile> P \<equiv> (true \<tturnstile> P)"
 
 translations
@@ -29,7 +31,31 @@ lemma sNotI: "\<Gamma> \<and> P \<tturnstile> false \<Longrightarrow> \<Gamma> \
 lemma sConjI: "\<lbrakk> \<Gamma> \<tturnstile> P; \<Gamma> \<tturnstile> Q \<rbrakk> \<Longrightarrow> \<Gamma> \<tturnstile> P \<and> Q"
   by pred_auto
 
-lemma sImplI: "\<lbrakk> (\<Gamma> \<and> P) \<tturnstile> Q \<rbrakk> \<Longrightarrow> \<Gamma> \<tturnstile> (P \<Rightarrow> Q)"
-  by pred_auto
+lemma sImplI: "\<lbrakk> P \<and> \<Gamma> \<tturnstile> Q \<rbrakk> \<Longrightarrow> \<Gamma> \<tturnstile> (P \<Rightarrow> Q)"
+  by pred_auto 
+
+lemma sAsmDisj: 
+  "\<lbrakk> A \<tturnstile> C; B \<tturnstile> C \<rbrakk> \<Longrightarrow> A \<or> B \<tturnstile> C"
+  by (rel_auto)
+
+lemma sDisjI1: "P \<tturnstile> Q \<Longrightarrow> P \<tturnstile> (Q \<or> R)"
+  by (rel_auto)
+
+lemma sDisjI2: "P \<tturnstile> R \<Longrightarrow> P \<tturnstile> (Q \<or> R)"
+  by (rel_auto)
+
+lemma sVarEqI:
+  assumes "wb_lens x" "(&x = v \<and> P) \<tturnstile> (Q\<lbrakk>v/&x\<rbrakk>)"
+  shows "(&x = v \<and> P) \<tturnstile> Q"
+  using assms by (rel_simp, metis wb_lens.get_put)
+
+lemma sWk: "\<lbrakk> `Q \<Rightarrow> P`; P \<tturnstile> R \<rbrakk> \<Longrightarrow> Q \<tturnstile> R"
+  by (rel_auto)
+
+lemma sWk1: "P \<tturnstile> R \<Longrightarrow> P \<and> Q \<tturnstile> R"
+  by (rel_auto)
+
+lemma sWk2: "Q \<tturnstile> R \<Longrightarrow> P \<and> Q \<tturnstile> R"
+  by (rel_auto)
 
 end
